src/Dafny/examples/fs/fs.dfy
@@ -1,0 +1,230 @@
+include "../../util/marshal.i.dfy"
+include "../../jrnl/jrnl.s.dfy"
+
+// NOTE: this module, unlike the others in this development, is not intended to
+// be opened
+//
+// NOTE: factoring out Inode to a separate file made this file much _slower_ for
+// some reason
+module Inode {
+  import opened Machine
+  import opened Collections
+  import opened ByteSlice
+  import opened Marshal
+
+  datatype Inode = Mk(sz: uint64, blks: seq<uint64>)
+
+  function method div_roundup(x: nat, k: nat): nat
+    requires k >= 1
+  {
+    (x + (k-1)) / k
+  }
+
+  predicate Valid(i:Inode)
+  {
+    var blks_ := i.blks;
+    // only direct blocks
+    && |blks_| == 15
+    && i.sz as nat <= |blks_| * 4096
+    && unique(blks_[..div_roundup(i.sz as nat, 4096)])
+  }
+
+  function inode_enc(i: Inode): seq<Encodable>
+  {
+    [EncUInt64(i.sz)] + seq_fmap(blkno => EncUInt64(blkno), i.blks)
+  }
+
+  function enc(i: Inode): seq<byte>
+  {
+    seq_encode(inode_enc(i))
+  }
+
+  const zero: Inode := Mk(0, repeat(0 as uint64, 15));
+
+  lemma zero_encoding()
+    ensures Valid(zero)
+    ensures repeat(0 as byte, 128) == enc(zero)
+  {
+    assert inode_enc(zero) == [EncUInt64(0)] + repeat(EncUInt64(0), 15);
+    assert inode_enc(zero) == repeat(EncUInt64(0), 16);
+    // TODO: need to assume this about little-endian encoding
+    assume enc_encode(EncUInt64(0)) == repeat(0 as byte, 8);
+    // TODO: prove this eventually
+    assume false;
+  }
+
+  method encode_ino(i: Inode) returns (bs:Bytes)
+    modifies {}
+    requires Valid(i)
+    ensures fresh(bs)
+    ensures bs.data == enc(i)
+  {
+    var enc := new Encoder(128);
+    enc.PutInt(i.sz);
+    var k: nat := 0;
+    while k < 15
+      modifies enc.Repr
+      invariant enc.Valid()
+      invariant 0 <= k <= 15
+      invariant enc.bytes_left() == 128 - ((k+1)*8)
+      invariant enc.enc ==
+      [EncUInt64(i.sz)] +
+      seq_fmap(blkno => EncUInt64(blkno), i.blks[..k])
+    {
+      enc.PutInt(i.blks[k]);
+      k := k + 1;
+    }
+    assert i.blks[..15] == i.blks;
+    bs := enc.FinishComplete();
+  }
+
+  method decode_ino(bs: Bytes, ghost i: Inode) returns (i': Inode)
+    modifies {}
+    requires bs.Valid()
+    requires Valid(i)
+    requires bs.data == enc(i)
+    ensures i' == i
+  {
+    var dec := new Decoder();
+    dec.Init(bs, inode_enc(i));
+    var sz := dec.GetInt(i.sz);
+    assert dec.enc == seq_fmap(blkno => EncUInt64(blkno), i.blks);
+
+    var blks: seq<uint64> := [];
+
+    var k: nat := 0;
+    while k < 15
+      modifies dec
+      invariant dec.Valid()
+      invariant Valid(i)
+      invariant 0 <= k <= 15
+      invariant blks == i.blks[..k]
+      invariant dec.enc == seq_fmap(blkno => EncUInt64(blkno), i.blks[k..])
+    {
+      var blk := dec.GetInt(i.blks[k]);
+      blks := blks + [blk];
+      k := k + 1;
+    }
+    return Mk(sz, blks);
+  }
+}
+
+module Fs {
+  import Inode
+  import opened Machine
+  import opened ByteSlice
+  import opened JrnlSpec
+  import opened Kinds
+  import opened Marshal
+
+  type Ino = uint64
+
+  // disk layout, in blocks:
+  //
+  // 513 for the jrnl
+  // 1 inode block (32 inodes)
+  // 1 bitmap block
+  // 4096*8 data blocks
+  const NumBlocks: nat := 513 + 1 + 1 + 4096*8
+
+  const InodeBlk: Blkno := 513
+  const DataAllocBlk: Blkno := 514
+  function method DataBlk(blkno: uint64): Addr
+    requires blkno as nat < 4096*8
+  {
+    Addr(513+2+blkno, 0)
+  }
+  function method InodeAddr(ino: Ino): (a:Addr)
+    requires ino < 32
+    ensures a.off < 4096*8
+  {
+    Addr(InodeBlk, ino*128*8)
+  }
+
+  const fs_kinds: map<Blkno, Kind> :=
+    // NOTE(tej): trigger annotation suppresses warning (there's nothing to
+    // trigger on here, but also nothing is necessary)
+    map blkno: Blkno {:trigger} |
+      513 <= blkno as nat < NumBlocks
+      :: (if blkno == InodeBlk
+      then KindInode
+      else if blkno == DataAllocBlk
+        then KindBit
+        else KindBlock) as Kind
+
+  lemma fs_kinds_valid()
+    ensures kindsValid(fs_kinds)
+  {}
+
+  class Filesys
+  {
+
+    // spec state
+    ghost var data: map<Ino, seq<byte>>;
+
+    // intermediate abstractions
+    ghost var inodes: map<Ino, Inode.Inode>;
+    ghost var block_used: map<Blkno, bool>;
+    ghost var data_block: map<Blkno, seq<byte>>;
+
+    var jrnl: Jrnl;
+    var balloc: Allocator;
+
+    static predicate ValidState(jrnl: Jrnl, data: map<Ino, seq<byte>>)
+      reads jrnl
+    {
+      && jrnl.Valid()
+      // TODO: eventually everything in Valid should go here (but this is
+      // annoying because we're going to be adding several ghost fields to Filesys)
+    }
+
+    predicate Valid()
+      reads this, jrnl
+    {
+      && ValidState(jrnl, data)
+      && jrnl.kinds == fs_kinds
+      && (forall ino: Ino | ino < 32 ::
+        && ino in inodes
+        && Inode.Valid(inodes[ino]))
+      && (forall ino: Ino | ino in data :: ino in inodes)
+      && (forall ino: Ino | ino in inodes ::
+        && ino in data
+        && inodes[ino].sz as nat == |data[ino]|)
+
+      && (forall blkno: uint64 :: blkno < 4096*8 <==> blkno in block_used)
+      && (forall blkno | blkno in block_used ::
+         jrnl.data[Addr(DataAllocBlk, blkno)] == ObjBit(block_used[blkno]))
+      // this is true but probably not useful
+      // && (forall blkno | blkno in block_used ::
+      //    jrnl.size(Addr(DataAllocBlk, blkno)) == 1)
+      && (forall blkno :: blkno in data_block <==> blkno < 4096*8)
+      && (forall blkno | blkno in data_block :: jrnl.data[DataBlk(blkno)] == ObjData(data_block[blkno]))
+
+      && (forall ino: Ino | ino < 32 :: jrnl.data[InodeAddr(ino)] == ObjData(Inode.enc(inodes[ino])))
+
+      && balloc.max == 4096*8
+    }
+
+    constructor(d: Disk)
+      ensures Valid()
+      ensures forall ino :: ino in this.data <==> ino < 513
+      ensures forall ino | ino in data :: data[ino] == []
+    {
+      var jrnl := NewJrnl(d, fs_kinds);
+      this.jrnl := jrnl;
+
+      var balloc := NewAllocator(4096*8);
+      balloc.MarkUsed(0);
+      this.balloc := balloc;
+      this.data := map ino: Ino {:trigger} | ino < 513 :: [];
+
+      this.inodes := map ino: Ino {:trigger} | ino < 513 :: Inode.zero;
+      Inode.zero_encoding();
+      this.block_used := map blkno: uint64 {:trigger} |
+        blkno < 4096*8 :: false;
+      this.data_block := map blkno: uint64 |
+        blkno < 4096*8 :: zeroObject(KindBlock).bs;
+    }
+  }
+
+}
